assets/strncat/strncat.v
@@ -2,64 +2,81 @@ Require Import Clightdefs.
 
 Local Open Scope Z_scope.
 
-Definition _dest : ident := 8%positive.
-Definition _i : ident := 5%positive.
-Definition _strncat : ident := 12%positive.
-Definition _n : ident := 10%positive.
-Definition ___builtin_annot_intval : ident := 3%positive.
+Definition ___builtin_fsqrt : ident := 16%positive.
+Definition _strlen : ident := 24%positive.
+Definition _i : ident := 22%positive.
+Definition ___builtin_read16_reversed : ident := 17%positive.
+Definition ___builtin_va_end : ident := 8%positive.
+Definition ___builtin_va_start : ident := 5%positive.
+Definition ___builtin_bswap : ident := 12%positive.
+Definition ___compcert_va_int64 : ident := 10%positive.
+Definition ___builtin_annot : ident := 3%positive.
 Definition ___builtin_memcpy_aligned : ident := 2%positive.
 Definition ___builtin_fabs : ident := 1%positive.
-Definition _c : ident := 6%positive.
-Definition _dest_len : ident := 11%positive.
-Definition _s : ident := 4%positive.
-Definition _strlen : ident := 7%positive.
-Definition _src : ident := 9%positive.
-Definition _main : ident := 13%positive.
-Definition _dest_len' : ident := 14%positive.
+Definition ___builtin_bswap16 : ident := 14%positive.
+Definition ___builtin_va_arg : ident := 6%positive.
+Definition _src : ident := 26%positive.
+Definition ___builtin_write16_reversed : ident := 19%positive.
+Definition ___compcert_va_float64 : ident := 11%positive.
+Definition ___builtin_annot_intval : ident := 4%positive.
+Definition _dest_len : ident := 28%positive.
+Definition ___builtin_va_copy : ident := 7%positive.
+Definition _s : ident := 21%positive.
+Definition ___builtin_read32_reversed : ident := 18%positive.
+Definition ___compcert_va_int32 : ident := 9%positive.
+Definition ___builtin_bswap32 : ident := 13%positive.
+Definition _n : ident := 27%positive.
+Definition _dest : ident := 25%positive.
+Definition ___builtin_cntlz : ident := 15%positive.
+Definition _strncat : ident := 29%positive.
+Definition _main : ident := 30%positive.
+Definition _c : ident := 23%positive.
+Definition ___builtin_write32_reversed : ident := 20%positive.
+Definition _dest_len' : ident := 31%positive.
 
 
 Definition f_strlen := {|
   fn_return := tuint;
-  fn_params := ((_s, (tptr tuchar)) :: nil);
+  fn_callconv := cc_default;
+  fn_params := ((_s, (tptr tint)) :: nil);
   fn_vars := nil;
-  fn_temps := ((_i, tuint) :: (_c, tuchar) :: nil);
+  fn_temps := ((_i, tuint) :: (_c, tint) :: nil);
   fn_body :=
 (Ssequence
   (Sset _i (Econst_int (Int.repr 0) tint))
   (Ssequence
     (Sset _c
-      (Ecast
-        (Ederef
-          (Ebinop Oadd (Etempvar _s (tptr tuchar)) (Etempvar _i tuint)
-            (tptr tuchar)) tuchar) tuchar))
+      (Ederef
+        (Ebinop Oadd (Etempvar _s (tptr tint)) (Etempvar _i tuint)
+          (tptr tint)) tint))
     (Ssequence
       (Swhile
-        (Ebinop One (Econst_int (Int.repr 0) tint) (Etempvar _c tuchar) tint)
+        (Ebinop One (Econst_int (Int.repr 0) tint) (Etempvar _c tint) tint)
         (Ssequence
           (Sset _i
             (Ebinop Oadd (Etempvar _i tuint) (Econst_int (Int.repr 1) tint)
               tuint))
           (Sset _c
-            (Ecast
-              (Ederef
-                (Ebinop Oadd (Etempvar _s (tptr tuchar)) (Etempvar _i tuint)
-                  (tptr tuchar)) tuchar) tuchar))))
+            (Ederef
+              (Ebinop Oadd (Etempvar _s (tptr tint)) (Etempvar _i tuint)
+                (tptr tint)) tint))))
       (Sreturn (Some (Etempvar _i tuint))))))
 |}.
 
 Definition f_strncat := {|
-  fn_return := (tptr tuchar);
-  fn_params := ((_dest, (tptr tuchar)) :: (_src, (tptr tuchar)) ::
-                (_n, tuint) :: nil);
+  fn_return := (tptr tint);
+  fn_callconv := cc_default;
+  fn_params := ((_dest, (tptr tint)) :: (_src, (tptr tint)) :: (_n, tuint) ::
+                nil);
   fn_vars := nil;
-  fn_temps := ((_dest_len, tuint) :: (_i, tuint) :: (15%positive, tint) ::
+  fn_temps := ((_dest_len, tuint) :: (_i, tuint) :: (32%positive, tint) ::
                (_dest_len', tuint) :: nil);
   fn_body :=
 (Ssequence
   (Ssequence
     (Scall (Some _dest_len')
-      (Evar _strlen (Tfunction (Tcons (tptr tuchar) Tnil) tuint))
-      ((Etempvar _dest (tptr tuchar)) :: nil))
+      (Evar _strlen (Tfunction (Tcons (tptr tint) Tnil) tuint cc_default))
+      ((Etempvar _dest (tptr tint)) :: nil))
     (Sset _dest_len (Etempvar _dest_len' tuint)))
   (Ssequence
     (Ssequence
@@ -70,55 +87,131 @@ Definition f_strncat := {|
             (Sifthenelse (Ebinop Olt (Etempvar _i tuint) (Etempvar _n tuint)
                            tint)
               (Ssequence
-                (Sset 15%positive
+                (Sset 32%positive
                   (Ecast
                     (Ebinop One
                       (Ederef
-                        (Ebinop Oadd (Etempvar _src (tptr tuchar))
-                          (Etempvar _i tuint) (tptr tuchar)) tuchar)
+                        (Ebinop Oadd (Etempvar _src (tptr tint))
+                          (Etempvar _i tuint) (tptr tint)) tint)
                       (Econst_int (Int.repr 0) tint) tint) tbool))
-                (Sset 15%positive (Ecast (Etempvar 15%positive tbool) tint)))
-              (Sset 15%positive (Econst_int (Int.repr 0) tint)))
-            (Sifthenelse (Etempvar 15%positive tint) Sskip Sbreak))
+                (Sset 32%positive (Ecast (Etempvar 32%positive tbool) tint)))
+              (Sset 32%positive (Econst_int (Int.repr 0) tint)))
+            (Sifthenelse (Etempvar 32%positive tint) Sskip Sbreak))
           (Sassign
             (Ederef
-              (Ebinop Oadd (Etempvar _dest (tptr tuchar))
+              (Ebinop Oadd (Etempvar _dest (tptr tint))
                 (Ebinop Oadd (Etempvar _dest_len tuint) (Etempvar _i tuint)
-                  tuint) (tptr tuchar)) tuchar)
+                  tuint) (tptr tint)) tint)
             (Ederef
-              (Ebinop Oadd (Etempvar _src (tptr tuchar)) (Etempvar _i tuint)
-                (tptr tuchar)) tuchar)))
+              (Ebinop Oadd (Etempvar _src (tptr tint)) (Etempvar _i tuint)
+                (tptr tint)) tint)))
         (Sset _i
           (Ebinop Oadd (Etempvar _i tuint) (Econst_int (Int.repr 1) tint)
             tuint))))
     (Ssequence
       (Sassign
         (Ederef
-          (Ebinop Oadd (Etempvar _dest (tptr tuchar))
+          (Ebinop Oadd (Etempvar _dest (tptr tint))
             (Ebinop Oadd (Etempvar _dest_len tuint) (Etempvar _i tuint)
-              tuint) (tptr tuchar)) tuchar) (Econst_int (Int.repr 0) tint))
-      (Sreturn (Some (Etempvar _dest (tptr tuchar)))))))
+              tuint) (tptr tint)) tint) (Econst_int (Int.repr 0) tint))
+      (Sreturn (Some (Etempvar _dest (tptr tint)))))))
 |}.
 
 Definition prog : Clight.program := {|
 prog_defs :=
 ((___builtin_fabs,
    Gfun(External (EF_builtin ___builtin_fabs
-                   (mksignature (AST.Tfloat :: nil) (Some AST.Tfloat)))
-     (Tcons tdouble Tnil) tdouble)) ::
+                   (mksignature (AST.Tfloat :: nil) (Some AST.Tfloat)
+                     cc_default)) (Tcons tdouble Tnil) tdouble cc_default)) ::
  (___builtin_memcpy_aligned,
    Gfun(External (EF_builtin ___builtin_memcpy_aligned
                    (mksignature
                      (AST.Tint :: AST.Tint :: AST.Tint :: AST.Tint :: nil)
-                     None))
+                     None cc_default))
      (Tcons (tptr tvoid)
-       (Tcons (tptr tvoid) (Tcons tuint (Tcons tuint Tnil)))) tvoid)) ::
+       (Tcons (tptr tvoid) (Tcons tuint (Tcons tuint Tnil)))) tvoid
+     cc_default)) ::
+ (___builtin_annot,
+   Gfun(External (EF_builtin ___builtin_annot
+                   (mksignature (AST.Tint :: nil) None
+                     {|cc_vararg:=true; cc_structret:=false|}))
+     (Tcons (tptr tuchar) Tnil) tvoid
+     {|cc_vararg:=true; cc_structret:=false|})) ::
  (___builtin_annot_intval,
    Gfun(External (EF_builtin ___builtin_annot_intval
-                   (mksignature (AST.Tint :: AST.Tint :: nil)
-                     (Some AST.Tint)))
-     (Tcons (tptr tuchar) (Tcons tint Tnil)) tint)) ::
- (_strlen, Gfun(Internal f_strlen)) ::
+                   (mksignature (AST.Tint :: AST.Tint :: nil) (Some AST.Tint)
+                     cc_default)) (Tcons (tptr tuchar) (Tcons tint Tnil))
+     tint cc_default)) ::
+ (___builtin_va_start,
+   Gfun(External (EF_builtin ___builtin_va_start
+                   (mksignature (AST.Tint :: nil) None cc_default))
+     (Tcons (tptr tvoid) Tnil) tvoid cc_default)) ::
+ (___builtin_va_arg,
+   Gfun(External (EF_builtin ___builtin_va_arg
+                   (mksignature (AST.Tint :: AST.Tint :: nil) None
+                     cc_default)) (Tcons (tptr tvoid) (Tcons tuint Tnil))
+     tvoid cc_default)) ::
+ (___builtin_va_copy,
+   Gfun(External (EF_builtin ___builtin_va_copy
+                   (mksignature (AST.Tint :: AST.Tint :: nil) None
+                     cc_default))
+     (Tcons (tptr tvoid) (Tcons (tptr tvoid) Tnil)) tvoid cc_default)) ::
+ (___builtin_va_end,
+   Gfun(External (EF_builtin ___builtin_va_end
+                   (mksignature (AST.Tint :: nil) None cc_default))
+     (Tcons (tptr tvoid) Tnil) tvoid cc_default)) ::
+ (___compcert_va_int32,
+   Gfun(External (EF_external ___compcert_va_int32
+                   (mksignature (AST.Tint :: nil) (Some AST.Tint) cc_default))
+     (Tcons (tptr tvoid) Tnil) tuint cc_default)) ::
+ (___compcert_va_int64,
+   Gfun(External (EF_external ___compcert_va_int64
+                   (mksignature (AST.Tint :: nil) (Some AST.Tlong)
+                     cc_default)) (Tcons (tptr tvoid) Tnil) tulong
+     cc_default)) ::
+ (___compcert_va_float64,
+   Gfun(External (EF_external ___compcert_va_float64
+                   (mksignature (AST.Tint :: nil) (Some AST.Tfloat)
+                     cc_default)) (Tcons (tptr tvoid) Tnil) tdouble
+     cc_default)) ::
+ (___builtin_bswap,
+   Gfun(External (EF_builtin ___builtin_bswap
+                   (mksignature (AST.Tint :: nil) (Some AST.Tint) cc_default))
+     (Tcons tuint Tnil) tuint cc_default)) ::
+ (___builtin_bswap32,
+   Gfun(External (EF_builtin ___builtin_bswap32
+                   (mksignature (AST.Tint :: nil) (Some AST.Tint) cc_default))
+     (Tcons tuint Tnil) tuint cc_default)) ::
+ (___builtin_bswap16,
+   Gfun(External (EF_builtin ___builtin_bswap16
+                   (mksignature (AST.Tint :: nil) (Some AST.Tint) cc_default))
+     (Tcons tushort Tnil) tushort cc_default)) ::
+ (___builtin_cntlz,
+   Gfun(External (EF_builtin ___builtin_cntlz
+                   (mksignature (AST.Tint :: nil) (Some AST.Tint) cc_default))
+     (Tcons tuint Tnil) tuint cc_default)) ::
+ (___builtin_fsqrt,
+   Gfun(External (EF_builtin ___builtin_fsqrt
+                   (mksignature (AST.Tfloat :: nil) (Some AST.Tfloat)
+                     cc_default)) (Tcons tdouble Tnil) tdouble cc_default)) ::
+ (___builtin_read16_reversed,
+   Gfun(External (EF_builtin ___builtin_read16_reversed
+                   (mksignature (AST.Tint :: nil) (Some AST.Tint) cc_default))
+     (Tcons (tptr tushort) Tnil) tushort cc_default)) ::
+ (___builtin_read32_reversed,
+   Gfun(External (EF_builtin ___builtin_read32_reversed
+                   (mksignature (AST.Tint :: nil) (Some AST.Tint) cc_default))
+     (Tcons (tptr tuint) Tnil) tuint cc_default)) ::
+ (___builtin_write16_reversed,
+   Gfun(External (EF_builtin ___builtin_write16_reversed
+                   (mksignature (AST.Tint :: AST.Tint :: nil) None
+                     cc_default)) (Tcons (tptr tushort) (Tcons tushort Tnil))
+     tvoid cc_default)) ::
+ (___builtin_write32_reversed,
+   Gfun(External (EF_builtin ___builtin_write32_reversed
+                   (mksignature (AST.Tint :: AST.Tint :: nil) None
+                     cc_default)) (Tcons (tptr tuint) (Tcons tuint Tnil))
+     tvoid cc_default)) :: (_strlen, Gfun(Internal f_strlen)) ::
  (_strncat, Gfun(Internal f_strncat)) :: nil);
 prog_main := _main
 |}.
